basics of decompositions

src/si.v
@@ -3,8 +3,32 @@ From Paco Require Import paco.
 Require Import ST.src.stream ST.processes.process ST.src.st ST.types.local.
 Require Import String List.
 Import ListNotations.
+Import CoListNotations.
 Require Import Setoid.
 Require Import Morphisms.
+
+CoFixpoint st2siH (t: st): st :=
+  match t with
+    | st_receive p xs    =>
+      match xs with
+        | cocons (l,s,t') ys => st_receive p [|(l,s,st2siH t')|] 
+        | conil              => st_receive p conil
+      end
+    | st_send p xs => 
+       let cofix next xs :=
+        match xs with
+          | cocons (l,s,t') ys => cocons (l,s,st2siH t') (next ys)
+          | conil              => conil
+        end 
+      in st_send p (next xs) 
+    | _               => st_end
+  end.
+
+CoFixpoint next (xs: coseq(label*sort*st)) :=
+  match xs with
+    | cocons (l,s,t') ys => cocons (l,s,st2siH t') (next ys)
+    | conil              => conil
+  end.
 
 Inductive st2si (R: st -> st -> Prop): st -> st -> Prop :=
   | st2si_end: st2si R st_end st_end
@@ -13,12 +37,12 @@ Inductive st2si (R: st -> st -> Prop): st -> st -> Prop :=
                copathsel l s xs y ->
                st2si R (st_receive p (cocons (l,s,x) conil)) (st_receive p xs)
   | st2si_snd: forall p xs ys,
-               Forall2Co (fun u v => exists l s t l' s' t', u = (l,s,t) /\ v = (l',s',t') /\ R t t') ys xs ->
+               Forall2Co (fun u v => exists l s t t', u = (l,s,t) /\ v = (l,s,t') /\ R t t') ys xs ->
                st2si R (st_send p ys) (st_send p xs).
 
 Definition st2siC s1 s2 := paco2 (st2si) bot2 s1 s2.
 
-Lemma st2so_mon: monotone2 st2si.
+Lemma st2si_mon: monotone2 st2si.
 Proof. unfold monotone2.
        intros.
        induction IN; intros.
