subtyping/subtyping.v
@@ -43,4 +43,114 @@ Definition subltype (T T': local) := subtype (lt2st T) (lt2st T').
 
 (* Definition subltype2 (T T': local) (T1 T2: st) (P: lt2stC T T1) (Q: lt2stC T' T2) := subtype2 T1 T2. *)
 
+Lemma pahselExt: forall ys xs l s y,
+  copathsel l s ys y ->
+  (Forall2Co (fun u v : string * local.sort * st =>exists (l : string) (s : local.sort) (t t' : st), u = (l, s, t) /\ v = (l, s, t') /\ upaco2 st2so bot2 t t') ys xs) ->
+  exists u, copathsel l s xs u /\ st2soC y u.
+Proof. intros.
+       revert xs H0.
+       induction H; intros.
+       - pinversion H0. subst.
+         destruct H2 as (l1,(s1,(t1,(t2,(H8a,(H8b,H8c)))))).
+         inversion H8a. subst.
+         exists t2. split. constructor. destruct H8c; easy.
+         apply mon_f2Ho.
+       - pinversion H1.
+         subst.
+         destruct H4 as (l1,(s1,(t1,(t2,(H8a,(H8b,H8c)))))).
+         inversion H8a. subst.
+         apply IHcopathsel in H6.
+         destruct H6 as (u,(H6a,H6b)).
+         exists u. split.
+         constructor. easy. easy. easy.
+         apply mon_f2Ho.
+       - pinversion H1.
+         subst.
+         destruct H4 as (l1,(s1,(t1,(t2,(H8a,(H8b,H8c)))))).
+         inversion H8a. subst.
+         apply IHcopathsel in H6.
+         destruct H6 as (u,(H6a,H6b)).
+         exists u. split.
+         apply pselneqs. easy. easy. easy.
+         apply mon_f2Ho.
+Qed.
 
+Lemma so_siDec: forall x y z, st2soC x y -> st2siC z x -> st2sisoC z y.
+Proof. pcofix CIH.
+       intros.
+       pinversion H0.
+       - subst. pinversion H1.
+         subst. pfold. constructor.
+         apply st2si_mon.
+       - subst. pinversion H1.
+         subst.
+         pinversion H5. subst.
+         destruct H7 as (l1,(s1,(t1,(t2,(H8a,(H8b,H8c)))))).
+         inversion H8b. subst.
+         pinversion H8. subst.
+         pfold. apply st2siso_snd with (y := y0).
+         right. apply CIH with (x := t2). easy. easy. easy.
+         apply mon_f2Ho.
+         apply mon_f2Ho.
+         apply st2si_mon.
+       - subst.
+         pinversion H1.
+         subst.
+         assert (exists u, copathsel l s xs u /\ st2soC y u).
+         { apply pahselExt with (xs := xs) in H6. easy. easy. }
+         destruct H2 as (u,(H3a,H3b)).
+         pfold.
+         apply st2siso_rcv with (y := u).
+         right. apply CIH with (x := y).
+         easy. easy.
+         easy.
+         apply st2si_mon.
+         apply st2so_mon.
+Qed.
+
+Lemma so_sisoDec: forall x y, wfC y -> st2soC x y -> st2sisoC (st2siH x) y.
+Proof. pcofix CIH.
+       intros.
+       pinversion H1. 
+       - subst. pfold. rewrite(st_eq(st2siH (end))). simpl.
+         constructor.
+       - subst. rewrite(st_eq(st2siH (p ! cocons (l, s, x0) conil))). simpl.
+         fold si.next.
+         rewrite(coseq_eq(si.next (cocons (l, s, x0) conil))). simpl.
+         rewrite(coseq_eq(si.next conil)). simpl.
+         pfold. apply st2siso_snd with (y := y0).
+         right.
+         apply CIH. admit. easy. easy.
+       - subst.
+         pinversion H. subst.
+         rewrite(st_eq(st2siH (p & conil))). simpl.
+         pfold. pinversion H0. subst.
+         easy.
+         apply mon_wfH.
+         subst.
+         destruct H2 as (l1,(s1,(t1,(t2,(H1a,(H1b,H1c)))))).
+         subst.
+         rewrite(st_eq(st2siH (p & cocons (l1, s1, t1) l))). simpl.
+         pfold. apply st2siso_rcv with (y := t2).
+         right. apply CIH.
+         pinversion H0. subst.
+         pinversion H6. subst.
+         destruct H7 as (l3,(s3,(t3,(H7a,H7b)))). inversion H7a. subst.
+         destruct H7b; easy.
+         apply mon_fHo.
+         apply mon_wfH.
+         destruct H1c; easy.
+         constructor.
+         apply mon_f2Ho.
+         apply st2so_mon.
+Admitted.
+
+Lemma si_sisoDec: forall x y, wfC y -> st2siC x y -> st2sisoC (st2soH x) y.
+Admitted.
+
+Lemma _3_15: forall T U V, wfC T -> st2soC U T -> st2siC V T -> exists W, st2siC W U /\ st2soC W V.
+Proof. intros.
+       apply so_sisoDec in H0; try easy.
+       apply si_sisoDec in H1; try easy.
+       exists (st2siH U). split. admit.
+Admitted.
